$$
\mu = \begin{cases}
\frac{1}{\tan \theta} \space \space \space \space \space \space \theta \in [0, \pi] \setminus \{\frac{\pi}{2}\}
\\
-\frac{1}{\tan \theta} \space \space \space \theta \in [\pi, 2\pi] \setminus \{\frac{3\pi}{2}\}
\end{cases}
$$

---

$$\frac{\mu}{\sqrt{1+\mu^2}} = \frac{\frac{1}{\tan \theta}}{\frac{\sqrt{\tan^2 \theta+1}}{\tan \theta}}$$
$$\space \space \space \space \space \space \space \space \space \space \space \space \space \space \space \space \space \space \space \space \space \space \space = \frac{1}{\sqrt{\frac{\sin^2 \theta+\cos^2 \theta}{\cos^2 \theta}}}$$
$$\space \space \space \space \space \space \space \space \space = \cos \theta$$

---

$$\cos^2 \theta = \frac{\sin^2 \theta}{\tan^2 \theta} = \frac{1-\cos^2 \theta}{\tan^2 \theta}$$
$$(\tan^2 \theta+1)\cos^2 \theta = 1$$
$$\cos \theta = \sqrt{\frac{1}{\tan^2 \theta + 1}}$$
$$\space \space \space \space \space \space \space \space = \frac{1}{\sqrt{\tan^2 \theta+1}}$$
$$\space \space \space \space \space \space \space \space \space \space \space \space \space \space \space = \frac{1}{\tan \theta \sqrt{1+\frac{1}{\tan^2 \theta}}}$$
$$\space \space = \frac{\mu}{\sqrt{1+\mu^2}}$$
